[Progress] Add user to exec semantics [Progress] Finish NI proofs for FileDisk

src/Framework/Layer/Core.v
@@ -8,12 +8,12 @@ Record Core :=
     token : Type;
     state : Type;
     operation : Type -> Type;
-    exec: forall T, token -> state -> operation T -> @Result state T -> Prop;
+    exec: forall T, user -> token -> state -> operation T -> @Result state T -> Prop;
     
     exec_deterministic_wrt_token :
-      forall o s T (p: operation T) ret1 ret2,
-        exec o s p ret1 ->
-        exec o s p ret2 ->
+      forall u o s T (p: operation T) ret1 ret2,
+        exec u o s p ret1 ->
+        exec u o s p ret2 ->
         ret1 = ret2;
   }.
 
