src/Framework/Layer/Language.v
@@ -22,51 +22,51 @@ Section Language.
   | Bind : forall T T', prog' T -> (T -> prog' T') -> prog' T'.
   
   Inductive exec' :
-    forall T, oracle' ->  state' -> prog' T -> @Result state' T -> Prop :=
+    forall T, user -> oracle' ->  state' -> prog' T -> @Result state' T -> Prop :=
   | ExecOp : 
-      forall T (p : O.(operation) T) o s s' r,
-        O.(exec) o s p (Finished s' r) ->
-        exec' [OpToken o] s (Op T p) (Finished s' r)
+      forall T (p : O.(operation) T) u o s s' r,
+        O.(exec) u o s p (Finished s' r) ->
+        exec' u [OpToken o] s (Op T p) (Finished s' r)
              
   | ExecRet :
-      forall d T (v: T),
-        exec' [Cont] d (Ret v) (Finished d v)
+      forall d T (v: T) u,
+        exec' u [Cont] d (Ret v) (Finished d v)
 
   | ExecBind :
       forall T T' (p1: prog' T) (p2: T -> prog' T')
-        o1 d1 d1' o2 r ret,
-        exec' o1 d1 p1 (Finished d1' r) ->
-        exec' o2 d1' (p2 r) ret ->
-        exec' (o1++o2) d1 (Bind p1 p2) ret
+        u o1 d1 d1' o2 r ret,
+        exec' u o1 d1 p1 (Finished d1' r) ->
+        exec' u o2 d1' (p2 r) ret ->
+        exec' u (o1++o2) d1 (Bind p1 p2) ret
 
   | ExecOpCrash : 
-      forall T (p : O.(operation) T) o s s',
-        O.(exec) o s p (Crashed s') ->
-        exec' [OpToken o] s (Op T p) (Crashed s')
+      forall T (p : O.(operation) T) u o s s',
+        O.(exec) u o s p (Crashed s') ->
+        exec' u [OpToken o] s (Op T p) (Crashed s')
              
   | ExecRetCrash :
-      forall T d (v: T),
-        exec' [Crash] d (Ret v) (Crashed d)
+      forall T d (v: T) u,
+        exec' u [Crash] d (Ret v) (Crashed d)
              
   | ExecBindCrash :
       forall T T' (p1: prog' T) (p2: T -> prog' T')
-        o1 o2 d1 d1',
-        exec' o1 d1 p1 (Crashed d1') ->
-        exec' (o1++o2) d1 (Bind p1 p2) (Crashed d1').
+        u o1 o2 d1 d1',
+        exec' u o1 d1 p1 (Crashed d1') ->
+        exec' u (o1++o2) d1 (Bind p1 p2) (Crashed d1').
 
   Inductive recovery_exec' :
-    forall T, list oracle' -> state' -> list (state' -> state') -> prog' T -> prog' unit -> @Recovery_Result state' T -> Prop :=
+    forall T, user -> list oracle' -> state' -> list (state' -> state') -> prog' T -> prog' unit -> @Recovery_Result state' T -> Prop :=
   | ExecFinished :
       forall T (p: prog' T) p_rec
-        o d d' t,
-        exec' o d p (Finished d' t) ->
-        recovery_exec' [o] d [] p p_rec (RFinished d' t)
+        u o d d' t,
+        exec' u o d p (Finished d' t) ->
+        recovery_exec' u [o] d [] p p_rec (RFinished d' t)
   | ExecRecovered :
       forall T (p: prog' T) p_rec
-        o lo d d' get_reboot_state l_grs ret,
-        exec' o d p (Crashed d') ->
-        recovery_exec' lo (get_reboot_state d') l_grs p_rec p_rec ret ->
-        recovery_exec' (o::lo) d (get_reboot_state::l_grs) p p_rec (Recovered (extract_state_r ret)).
+        u o lo d d' get_reboot_state l_grs ret,
+        exec' u o d p (Crashed d') ->
+        recovery_exec' u lo (get_reboot_state d') l_grs p_rec p_rec ret ->
+        recovery_exec' u (o::lo) d (get_reboot_state::l_grs) p p_rec (Recovered (extract_state_r ret)).
   
   Hint Constructors exec' : core.
 
@@ -84,7 +84,7 @@ End Language.
 
 Arguments Ret {O T}.
 Arguments Op O {T}.
-Hint Extern 1 (Language.exec _ _ _ (Op _ _) (Finished _ _)) => eapply (ExecOp _) : core.
+Hint Extern 1 (Language.exec _ _ _ _ (Op _ _) (Finished _ _)) => eapply (ExecOp _) : core.
 Notation "| p |" := (Op _ p)(at level 60).
 Notation "x <- p1 ; p2" := (Bind p1 (fun x => p2))(right associativity, at level 60).
 Notation "x <-| p1 ; p2" := (Bind (Op _ p1) (fun x => p2))(right associativity, at level 60).
@@ -95,9 +95,9 @@ Notation "x <-| p1 ; p2" := (Bind (Op _ p1) (fun x => p2))(right associativity, 
  (** Facts **)
 
 Lemma exec_finished_deterministic_prefix:
-  forall O (L: Language O) T (p: prog L T) o1 o2 o3 o4 s s1 s2 r1 r2,
-      exec L o1 s p (Finished s1 r1) ->
-      exec L o2 s p (Finished s2 r2) -> 
+  forall O (L: Language O) T (p: prog L T) u o1 o2 o3 o4 s s1 s2 r1 r2,
+      exec L u o1 s p (Finished s1 r1) ->
+      exec L u o2 s p (Finished s2 r2) -> 
       o1 ++ o3 = o2 ++ o4 ->
       o1 = o2 /\ s1 = s2 /\ r1 = r2.
 Proof.
@@ -106,27 +106,27 @@ Proof.
     simpl in *; cleanup;
     simpl; eauto; try solve [intuition].
   
-  eapply O.(exec_deterministic_wrt_token) in H7; eauto; cleanup; eauto.
+  eapply O.(exec_deterministic_wrt_token) in H8; eauto; cleanup; eauto.
   
   repeat rewrite <- app_assoc in H2.
-  specialize IHp with (1:= H8)(2:= H17)(3:=H2); cleanup.
-  specialize H with (1:= H11)(2:= H20)(3:=H2); cleanup; eauto.
+  specialize IHp with (1:= H9)(2:= H19)(3:=H2); cleanup.
+  specialize H with (1:= H12)(2:= H22)(3:=H2); cleanup; eauto.
 Qed.
 
 Lemma finished_not_crashed_oracle_prefix:
-  forall O (L: Language O) T (p: prog L T) o1 o2 o3 o4 s s1 s2 r1,
-    exec L o1 s p (Finished s1 r1) ->
+  forall O (L: Language O) T (p: prog L T) u o1 o2 o3 o4 s s1 s2 r1,
+    exec L u o1 s p (Finished s1 r1) ->
     o1 ++ o3 = o2 ++ o4 ->
-    ~exec L o2 s p (Crashed s2).
+    ~exec L u o2 s p (Crashed s2).
 Proof.
   unfold not; induction p; simpl; intros;
   (try inversion H; try inversion H0; try inversion H1;
     try inversion H2; simpl in *; cleanup);
   simpl in *; cleanup; simpl; eauto.
-  eapply exec_deterministic_wrt_token in H7; eauto; cleanup.
+  eapply exec_deterministic_wrt_token in H8; eauto; cleanup.
   -
     repeat rewrite <- app_assoc in H1; eauto.
-    eapply exec_finished_deterministic_prefix in H8; eauto; cleanup; eauto.
+    eapply exec_finished_deterministic_prefix in H9; eauto; cleanup; eauto.
   -
     repeat rewrite <- app_assoc in H1; eauto.
     Unshelve.
@@ -134,29 +134,29 @@ Proof.
 Qed.
 
 Lemma finished_not_crashed_oracle_app:
-  forall O (L: Language O) T (p: prog L T) o1 o2 s s1 s2 r1,
-    exec L o1 s p (Finished s1 r1) ->
-    ~exec L (o1++o2) s p (Crashed s2).
+  forall O (L: Language O) T (p: prog L T) u o1 o2 s s1 s2 r1,
+    exec L u o1 s p (Finished s1 r1) ->
+    ~exec L u (o1++o2) s p (Crashed s2).
 Proof.
   unfold not; induction p; simpl; intros;
   (try inversion H; try inversion H0; try inversion H1;
     try inversion H2; simpl in *; cleanup);
   simpl in *; cleanup; simpl; eauto.
-  eapply exec_deterministic_wrt_token in H6; eauto; cleanup.
+  eapply exec_deterministic_wrt_token in H7; eauto; cleanup.
 
-  - rewrite <- app_assoc in H11; eauto.
-    eapply exec_finished_deterministic_prefix in H7; eauto; cleanup; eauto.
+  - rewrite <- app_assoc in H12; eauto.
+    eapply exec_finished_deterministic_prefix in H8; eauto; cleanup; eauto.
     
-  - rewrite <- app_assoc in H11; eauto.
-    clear H1; eapply finished_not_crashed_oracle_prefix in H7; eauto.
+  - rewrite <- app_assoc in H12; eauto.
+    clear H1; eapply finished_not_crashed_oracle_prefix in H8; eauto.
     Unshelve.
     all: eauto.  
 Qed.
 
 Lemma exec_deterministic_wrt_oracle_prefix:
-      forall O (L: Language O) T (p: prog L T) o1 o2 x1 x2 s ret1 ret2,
-      exec L o1 s p ret1 -> 
-      exec L x1 s p ret2 ->
+      forall O (L: Language O) T (p: prog L T) u o1 o2 x1 x2 s ret1 ret2,
+      exec L u o1 s p ret1 -> 
+      exec L u x1 s p ret2 ->
       o1 ++ o2 = x1 ++ x2 ->
       ret1 = ret2.
     Proof.
@@ -168,32 +168,32 @@ Lemma exec_deterministic_wrt_oracle_prefix:
   -
     eapply O.(exec_deterministic_wrt_token); eauto.
   -
-    eapply O.(exec_deterministic_wrt_token) in H7; eauto; cleanup.
+    eapply O.(exec_deterministic_wrt_token) in H8; eauto; cleanup.
   -
-    eapply O.(exec_deterministic_wrt_token) in H7; eauto; cleanup.
+    eapply O.(exec_deterministic_wrt_token) in H8; eauto; cleanup.
   -
     eapply O.(exec_deterministic_wrt_token); eauto; cleanup.
   -
-    eapply exec_finished_deterministic_prefix in H8; eauto; cleanup; eauto.
+    eapply exec_finished_deterministic_prefix in H9; eauto; cleanup; eauto.
     repeat rewrite <- app_assoc in H2; cleanup; eauto.
     repeat rewrite <- app_assoc in H2; eauto.
   -
     repeat rewrite <- app_assoc in H2; eauto.
-    specialize IHp with (1:=H8)(2:=H16)(3:=H2); cleanup.
+    specialize IHp with (1:=H9)(2:=H18)(3:=H2); cleanup.
 
   - repeat rewrite <- app_assoc in H2.
-    specialize IHp with (1:=H7)(2:=H16)(3:=H2); cleanup.
+    specialize IHp with (1:=H8)(2:=H18)(3:=H2); cleanup.
   -
     repeat rewrite <- app_assoc in H2.
-    specialize IHp with (1:=H7)(2:=H15)(3:=H2); cleanup; eauto.
+    specialize IHp with (1:=H8)(2:=H17)(3:=H2); cleanup; eauto.
     Unshelve.
     eauto.
  Qed.
     
 Lemma exec_deterministic_wrt_oracle:
-  forall O (L: Language O) T (p: prog L T) o s r1 r2,
-      exec L o s p r1 ->
-      exec L o s p r2 ->
+  forall O (L: Language O) T (p: prog L T) u o s r1 r2,
+      exec L u o s p r1 ->
+      exec L u o s p r2 ->
       r1 = r2.
 Proof.
   intros.
@@ -203,16 +203,16 @@ Proof.
 Qed.
 
 Lemma recovery_exec_deterministic_wrt_reboot_state :
-  forall O (L: Language O) lo s T (p: L.(prog) T) rec l_get_reboot_state ret1 ret2,
-    recovery_exec L lo s l_get_reboot_state p rec ret1 ->
-    recovery_exec L lo s l_get_reboot_state p rec ret2 ->
+  forall O (L: Language O) u lo s T (p: L.(prog) T) rec l_get_reboot_state ret1 ret2,
+    recovery_exec L u lo s l_get_reboot_state p rec ret1 ->
+    recovery_exec L u lo s l_get_reboot_state p rec ret2 ->
     ret1 = ret2.
 Proof.
   induction 1; intros;  try repeat
                              match goal with
-                             | [H: exec' _ _ (Bind _ _) _ |- _ ] =>
+                             | [H: exec' _ _ _ (Bind _ _) _ |- _ ] =>
                                inversion H; clear H; simpl in *; cleanup
-                             | [H: recovery_exec _ _ _ _ _ _ _ |- _ ] =>
+                             | [H: recovery_exec _ _ _ _ _ _ _ _ |- _ ] =>
                                inversion H; clear H; simpl in *; cleanup
                              end.
   try solve [eapply exec_deterministic_wrt_oracle in H; eauto; cleanup; eauto].
