src/Framework/Simulation/Definitions.v
@@ -4,14 +4,14 @@ Record CoreRefinement {O_imp} (L_imp: Language O_imp) (O_abs: Core) :=
   {
     compile_core : forall T, O_abs.(Core.operation) T -> L_imp.(prog) T;
     refines_to_core: L_imp.(state) -> O_abs.(Core.state) -> Prop;
-    token_refines_to: forall T, L_imp.(state) -> O_abs.(Core.operation) T -> (L_imp.(state) -> L_imp.(state)) -> L_imp.(oracle) -> O_abs.(Core.token) -> Prop;
+    token_refines_to: forall T, user -> L_imp.(state) -> O_abs.(Core.operation) T -> (L_imp.(state) -> L_imp.(state)) -> L_imp.(oracle) -> O_abs.(Core.token) -> Prop;
   }.
 
 Record Refinement {O_imp O_abs} (L_imp: Language O_imp) (L_abs: Language O_abs) :=
   {
     compile : forall T, L_abs.(prog) T -> L_imp.(prog) T;
     refines_to: L_imp.(state) -> L_abs.(state) -> Prop;
-    oracle_refines_to: forall T, L_imp.(state) -> L_abs.(prog) T -> (L_imp.(state) -> L_imp.(state)) -> L_imp.(oracle) -> L_abs.(oracle) -> Prop;
+    oracle_refines_to: forall T, user -> L_imp.(state) -> L_abs.(prog) T -> (L_imp.(state) -> L_imp.(state)) -> L_imp.(oracle) -> L_abs.(oracle) -> Prop;
   }.
 
 Arguments Build_CoreRefinement {_ _ _}.
@@ -31,31 +31,31 @@ Section Relations.
   Variable R : Refinement L_imp L_abs.
   
   Fixpoint recovery_oracles_refine_to {T}
-           (s: L_imp.(state)) (p_abs: L_abs.(prog) T) (rec_abs: L_abs.(prog) unit)
+           (u: user) (s: L_imp.(state)) (p_abs: L_abs.(prog) T) (rec_abs: L_abs.(prog) unit)
            (l_get_reboot_state_imp: list (L_imp.(state) -> L_imp.(state)))
            (lo_imp: list L_imp.(oracle)) (lo_abs: list L_abs.(oracle)) {struct lo_imp} :=
     match lo_imp, lo_abs with
     | o_imp :: loi, o_abs :: loa =>
       length lo_imp = length lo_abs /\
       (forall s' t,
-         L_imp.(exec) o_imp s (R.(compile) p_abs) (Finished s' t) ->
-         R.(oracle_refines_to) s p_abs (fun s => s) o_imp o_abs) /\
+         L_imp.(exec) u o_imp s (R.(compile) p_abs) (Finished s' t) ->
+         R.(oracle_refines_to) u s p_abs (fun s => s) o_imp o_abs) /\
       (forall s',
-         L_imp.(exec) o_imp s (R.(compile) p_abs) (Crashed s') ->
+         L_imp.(exec) u o_imp s (R.(compile) p_abs) (Crashed s') ->
          match l_get_reboot_state_imp with
          | get_reboot_state_imp :: lgrsi =>
-           R.(oracle_refines_to) s p_abs get_reboot_state_imp o_imp o_abs /\
-           recovery_oracles_refine_to (get_reboot_state_imp s') rec_abs rec_abs lgrsi loi loa
+           R.(oracle_refines_to) u s p_abs get_reboot_state_imp o_imp o_abs /\
+           recovery_oracles_refine_to u (get_reboot_state_imp s') rec_abs rec_abs lgrsi loi loa
          | _ => False
          end)
     | _, _ => False
     end.
 
-Definition abstract_oracles_exist_wrt Rel {T} (p_abs: L_abs.(prog) T) rec_abs l_get_reboot_state :=
+Definition abstract_oracles_exist_wrt Rel (u: user) {T} (p_abs: L_abs.(prog) T) rec_abs l_get_reboot_state :=
   forall l_oi si si',
     (exists sa: L_abs.(state), Rel si sa) -> 
-    L_imp.(recovery_exec) l_oi si l_get_reboot_state (R.(compile) p_abs) (R.(compile) rec_abs) si' ->
-    exists l_oa, recovery_oracles_refine_to si p_abs rec_abs l_get_reboot_state l_oi l_oa.
+    L_imp.(recovery_exec) u l_oi si l_get_reboot_state (R.(compile) p_abs) (R.(compile) rec_abs) si' ->
+    exists l_oa, recovery_oracles_refine_to u si p_abs rec_abs l_get_reboot_state l_oi l_oa.
 
 (** 
 A relation that takes 
@@ -86,22 +86,22 @@ Definition refines_to_valid
     valid_state_abs sa.
 
 
-Definition exec_compiled_preserves_validity  {T} (p_abs: L_abs.(prog) T) rec_abs l_get_reboot_state (valid_state: L_imp.(state) -> Prop) := 
+Definition exec_compiled_preserves_validity  {T} (u: user)(p_abs: L_abs.(prog) T) rec_abs l_get_reboot_state (valid_state: L_imp.(state) -> Prop) := 
     forall l_oi s ret,
       valid_state s ->
-      L_imp.(recovery_exec) l_oi s l_get_reboot_state (R.(compile) p_abs) (R.(compile) rec_abs) ret ->
+      L_imp.(recovery_exec) u l_oi s l_get_reboot_state (R.(compile) p_abs) (R.(compile) rec_abs) ret ->
       valid_state (extract_state_r ret).
 
 
 Definition oracle_refines_to_same_from_related
-            {T} (p1_abs p2_abs: L_abs.(prog) T)
+            (u: user) {T} (p1_abs p2_abs: L_abs.(prog) T)
             rec_abs
             l_get_reboot_state_imp
            (related_states_abs: L_abs.(state) -> L_abs.(state) -> Prop) :=
   forall l_o_imp l_o_abs l_o_abs' s1_imp s2_imp,
     refines_to_related related_states_abs s1_imp s2_imp ->
-    recovery_oracles_refine_to s1_imp p1_abs rec_abs l_get_reboot_state_imp l_o_imp l_o_abs ->
-    recovery_oracles_refine_to s2_imp p2_abs rec_abs l_get_reboot_state_imp l_o_imp l_o_abs' ->
+    recovery_oracles_refine_to u s1_imp p1_abs rec_abs l_get_reboot_state_imp l_o_imp l_o_abs ->
+    recovery_oracles_refine_to u s2_imp p2_abs rec_abs l_get_reboot_state_imp l_o_imp l_o_abs' ->
 l_o_abs = l_o_abs'.
 
 (** Self Simulation **)
@@ -111,25 +111,26 @@ l_o_abs = l_o_abs'.
   R: This is the actual simulation relation
 **)
 
-Definition SelfSimulation {T} (p1 p2: L_abs.(prog) T)
+Definition SelfSimulation (u: user) {T} (p1 p2: L_abs.(prog) T)
        (rec: L_abs.(prog) unit)
        (valid_state: L_abs.(state) -> Prop)
        (R: L_abs.(state) -> L_abs.(state) -> Prop)
+       (cond: user -> Prop)
        l_get_reboot_state :=
   forall lo s1 s1',
-    L_abs.(recovery_exec) lo s1 l_get_reboot_state p1 rec s1' ->
+    L_abs.(recovery_exec) u lo s1 l_get_reboot_state p1 rec s1' ->
     valid_state s1 ->
     forall s2,
     valid_state s2 ->
     R s1 s2 ->
     exists s2',
-      L_abs.(recovery_exec) lo s2 l_get_reboot_state p2 rec s2' /\
+      L_abs.(recovery_exec) u lo s2 l_get_reboot_state p2 rec s2' /\
       R (extract_state_r s1') (extract_state_r s2') /\
-      extract_ret_r s1' = extract_ret_r s2' /\
+      (cond u -> extract_ret_r s1' = extract_ret_r s2') /\
       valid_state (extract_state_r s1') /\
       valid_state (extract_state_r s2').
 
-Definition SelfSimulation_Exists  {T} (p1 p2: L_abs.(prog) T)
+Definition SelfSimulation_Exists u {T} (p1 p2: L_abs.(prog) T)
            (rec: L_abs.(prog) unit)
            (valid_state: L_abs.(state) -> Prop)
            (R: L_abs.(state) -> L_abs.(state) -> Prop)
@@ -137,35 +138,36 @@ Definition SelfSimulation_Exists  {T} (p1 p2: L_abs.(prog) T)
   forall s1 s1' s2 lo,
     valid_state s1 ->
     valid_state s2 -> 
-    L_abs.(recovery_exec) lo s1 l_get_reboot_state p1 rec s1' ->
+    L_abs.(recovery_exec) u lo s1 l_get_reboot_state p1 rec s1' ->
     R s1 s2 ->
     exists s2', 
-      L_abs.(recovery_exec) lo s2 l_get_reboot_state p2 rec s2'.
+      L_abs.(recovery_exec) u lo s2 l_get_reboot_state p2 rec s2'.
 
-Definition SelfSimulation_Weak {T} (p1 p2: L_abs.(prog) T)
+Definition SelfSimulation_Weak u {T} (p1 p2: L_abs.(prog) T)
            (rec: L_abs.(prog) unit)
            (valid_state: L_abs.(state) -> Prop)
            (R: L_abs.(state) -> L_abs.(state) -> Prop)
+           (cond: user -> Prop)
            l_get_reboot_state :=
   forall lo s1 s1' s2 s2',
-    L_abs.(recovery_exec) lo s1 l_get_reboot_state p1 rec s1' ->
-    L_abs.(recovery_exec) lo s2 l_get_reboot_state p2 rec s2' ->
+    L_abs.(recovery_exec) u lo s1 l_get_reboot_state p1 rec s1' ->
+    L_abs.(recovery_exec) u lo s2 l_get_reboot_state p2 rec s2' ->
     valid_state s1 ->
     valid_state s2 ->
     R s1 s2 ->
     R (extract_state_r s1') (extract_state_r s2') /\
-    extract_ret_r s1' = extract_ret_r s2' /\
+    (cond u -> extract_ret_r s1' = extract_ret_r s2') /\
     valid_state (extract_state_r s1') /\
     valid_state (extract_state_r s2').
 
 Lemma Self_Simulation_Weak_to_Self_Simulation:
-  forall T (p1 p2: L_abs.(prog) T) R
-    valid_state rec l_get_reboot_state,
+  forall u T (p1 p2: L_abs.(prog) T) R
+    valid_state rec cond l_get_reboot_state,
 
-    SelfSimulation_Exists p1 p2 rec valid_state R l_get_reboot_state ->
-    SelfSimulation_Weak p1 p2 rec valid_state R l_get_reboot_state ->
+    SelfSimulation_Exists u p1 p2 rec valid_state R l_get_reboot_state ->
+    SelfSimulation_Weak u p1 p2 rec valid_state R cond l_get_reboot_state ->
     
-    SelfSimulation p1 p2 rec valid_state R l_get_reboot_state.
+    SelfSimulation u p1 p2 rec valid_state R cond l_get_reboot_state.
 Proof.
   unfold SelfSimulation_Exists, SelfSimulation_Weak, SelfSimulation; intros.
   edestruct H.
@@ -174,100 +176,101 @@ Proof.
 Qed.
 
 
-
 (** Simulation **)
 Definition SimulationForProgramGeneral
-           T (p_abs: L_abs.(prog) T) (rec_abs : L_abs.(prog) unit)
+           u T (p_abs: L_abs.(prog) T) (rec_abs : L_abs.(prog) unit)
            l_get_reboot_state_imp
            l_get_reboot_state_abs
            R_begin R_end :=
   forall l_o_imp l_o_abs s_imp s_abs,
-    recovery_oracles_refine_to s_imp p_abs rec_abs l_get_reboot_state_imp l_o_imp l_o_abs ->
+    recovery_oracles_refine_to u s_imp p_abs rec_abs l_get_reboot_state_imp l_o_imp l_o_abs ->
     R_begin s_imp s_abs ->
 
     (forall s_imp',
-       L_imp.(recovery_exec) l_o_imp s_imp
+       L_imp.(recovery_exec) u l_o_imp s_imp
                              l_get_reboot_state_imp (R.(compile) p_abs)
                              (R.(compile) rec_abs) s_imp' ->
        exists s_abs',
-         L_abs.(recovery_exec) l_o_abs s_abs l_get_reboot_state_abs p_abs rec_abs s_abs' /\
+         L_abs.(recovery_exec) u l_o_abs s_abs l_get_reboot_state_abs p_abs rec_abs s_abs' /\
          R_end (extract_state_r s_imp') (extract_state_r s_abs') /\
          extract_ret_r s_imp' = extract_ret_r s_abs'
     ).
 
- Definition SimulationForProgram T (p_abs: L_abs.(prog) T) (rec_abs : L_abs.(prog) unit)
+ Definition SimulationForProgram u T (p_abs: L_abs.(prog) T) (rec_abs : L_abs.(prog) unit)
            l_get_reboot_state_imp
            l_get_reboot_state_abs :=
-    SimulationForProgramGeneral T p_abs rec_abs l_get_reboot_state_imp l_get_reboot_state_abs R.(refines_to) R.(refines_to).
+    SimulationForProgramGeneral u T p_abs rec_abs l_get_reboot_state_imp l_get_reboot_state_abs R.(refines_to) R.(refines_to).
 
 Definition Simulation rec_abs l_get_reboot_state_imp l_get_reboot_state_abs
-    := forall T (p_abs: L_abs.(prog) T),
-         SimulationForProgram T p_abs rec_abs l_get_reboot_state_imp l_get_reboot_state_abs.
+    := forall u T (p_abs: L_abs.(prog) T),
+         SimulationForProgram u T p_abs rec_abs l_get_reboot_state_imp l_get_reboot_state_abs.
 
 End Relations.
 
-Arguments recovery_oracles_refine_to {_ _ _ _} _ {_}.
+Arguments recovery_oracles_refine_to {_ _ _ _} _ _ {_}.
 Arguments refines_to_related {_ _ _ _}.
 Arguments refines_to_valid {_ _ _ _}.
 Arguments exec_compiled_preserves_validity {_ _ _ _} _ {_}.
-Arguments abstract_oracles_exist_wrt {_ _ _ _} _ _ {_}.
-Arguments oracle_refines_to_same_from_related {_ _ _ _} _ {_}.
-Arguments SelfSimulation {_ _ _}.
-Arguments SelfSimulation_Weak {_ _ _}.
-Arguments SelfSimulation_Exists {_ _ _}.
+Arguments abstract_oracles_exist_wrt {_ _ _ _} _ _ _ {_}.
+Arguments oracle_refines_to_same_from_related {_ _ _ _} _ _ {_}.
+Arguments SelfSimulation {_ _} _ {_}.
+Arguments SelfSimulation_Weak {_ _} _ {_}.
+Arguments SelfSimulation_Exists {_ _} _ {_}.
 Arguments Simulation {_ _ _ _}.
-Arguments SimulationForProgram {_ _ _ _} _ {_}.
-
+Arguments SimulationForProgram {_ _ _ _} _ _ {_}.
 
 Lemma SS_transfer:
   forall O_imp O_abs (L_imp: Language O_imp) (L_abs: Language O_abs) (R: Refinement L_imp L_abs)
-    T (p1_abs p2_abs: L_abs.(prog) T)
+    u T (p1_abs p2_abs: L_abs.(prog) T)
       rec_abs
       l_get_reboot_state_imp
       l_get_reboot_state_abs
       equivalent_states_abs
-      valid_state_abs,
+      valid_state_abs
+      cond,
 
     SelfSimulation
-      p1_abs p2_abs
+      u p1_abs p2_abs
       rec_abs
       valid_state_abs
       equivalent_states_abs
+      cond
       l_get_reboot_state_abs ->
     
-    SimulationForProgram R p1_abs rec_abs 
+    SimulationForProgram R u p1_abs rec_abs 
       l_get_reboot_state_imp
       l_get_reboot_state_abs ->
 
-    SimulationForProgram R p2_abs rec_abs 
+    SimulationForProgram R u p2_abs rec_abs 
       l_get_reboot_state_imp
       l_get_reboot_state_abs ->
 
-    abstract_oracles_exist_wrt R R.(refines_to) p1_abs rec_abs l_get_reboot_state_imp ->
-    abstract_oracles_exist_wrt R R.(refines_to) p2_abs rec_abs l_get_reboot_state_imp ->
+    abstract_oracles_exist_wrt R R.(refines_to) u p1_abs rec_abs l_get_reboot_state_imp ->
+    abstract_oracles_exist_wrt R R.(refines_to) u p2_abs rec_abs l_get_reboot_state_imp ->
     
-    oracle_refines_to_same_from_related R p1_abs p2_abs rec_abs l_get_reboot_state_imp equivalent_states_abs ->
+    oracle_refines_to_same_from_related R u p1_abs p2_abs rec_abs l_get_reboot_state_imp equivalent_states_abs ->
 
     exec_compiled_preserves_validity R
-    p1_abs rec_abs l_get_reboot_state_imp
+    u p1_abs rec_abs l_get_reboot_state_imp
     (refines_to_valid R valid_state_abs) ->
 
     exec_compiled_preserves_validity R
-    p2_abs rec_abs l_get_reboot_state_imp
+    u p2_abs rec_abs l_get_reboot_state_imp
     (refines_to_valid R valid_state_abs) ->
 
-    SelfSimulation_Exists (compile R p1_abs)
+    SelfSimulation_Exists u (compile R p1_abs)
     (compile R p2_abs) (compile R rec_abs)
     (refines_to_valid R valid_state_abs)
     (refines_to_related R equivalent_states_abs)
     l_get_reboot_state_imp ->
     
     SelfSimulation
-      (R.(compile) p1_abs)
+      u (R.(compile) p1_abs)
       (R.(compile) p2_abs)
       (R.(compile) rec_abs)
       (refines_to_valid R valid_state_abs)
       (refines_to_related R equivalent_states_abs)
+      cond
       l_get_reboot_state_imp.
 Proof.
 
@@ -280,19 +283,19 @@ Proof.
   (* unfold refines_to_valid, refines_to_related in *; cleanup. *)
 
   match goal with
-  | [H: recovery_exec _ _ _ _ (compile _ ?p1) _ _,
-     H0: recovery_exec _ _ _ _ (compile _ ?p2) _ _,
-     H1: abstract_oracles_exist_wrt _ _ ?p1 _ _,
-     H2: abstract_oracles_exist_wrt _ _ ?p2 _ _ |- _ ] =>
+  | [H: recovery_exec _ _ _ _ _ (compile _ ?p1) _ _,
+     H0: recovery_exec _ _ _ _ _ (compile _ ?p2) _ _,
+     H1: abstract_oracles_exist_wrt _ _ _ ?p1 _ _,
+     H2: abstract_oracles_exist_wrt _ _ _ ?p2 _ _ |- _ ] =>
     eapply_fresh H1 in H; eauto; cleanup;
     eapply_fresh H2 in H0; eauto; cleanup;
     try solve [ unfold refines_to_valid, refines_to_related in *; cleanup; eauto]
   end.
   
   match goal with
-  | [H: recovery_oracles_refine_to _ _ _ _ _ _ _,
-     H0: recovery_oracles_refine_to _ _ _ _ _ _ _,
-     H1: oracle_refines_to_same_from_related _ _ _ _ _ _ |- _ ] =>
+  | [H: recovery_oracles_refine_to _ _ _ _ _ _ _ _,
+     H0: recovery_oracles_refine_to _ _ _ _ _ _ _ _,
+     H1: oracle_refines_to_same_from_related _ _ _ _ _ _ _ |- _ ] =>
     eapply_fresh H1 in H0; eauto; cleanup
   end.
   
@@ -300,10 +303,10 @@ Proof.
   unfold refines_to_related in *; cleanup.
   
   match goal with
-  | [H: recovery_exec _ _ _ _ (compile _ ?p1) _ _,
-     H0: recovery_exec _ _ _ _ (compile _ ?p2) _ _,
-     H1: SimulationForProgram _ ?p1 _ _ _,
-     H2: SimulationForProgram _ ?p2 _ _ _ |- _ ] =>
+  | [H: recovery_exec _ _ _ _ _ (compile _ ?p1) _ _,
+     H0: recovery_exec _ _ _ _ _ (compile _ ?p2) _ _,
+     H1: SimulationForProgram _ _ ?p1 _ _ _,
+     H2: SimulationForProgram _ _ ?p2 _ _ _ |- _ ] =>
     eapply_fresh H1 in H; eauto; cleanup;
     eapply_fresh H2 in H0; eauto; cleanup
   end.
@@ -311,9 +314,9 @@ Proof.
 
   (** Use self_simulation to generate second abs execution from s2 **)
   match goal with
-  | [H: recovery_exec L_abs _ _ _ p1_abs _ _,
-     H0: recovery_exec L_abs _ _ _ _ _ _,
-     H1: SelfSimulation _ _ _ _ _ _,
+  | [H: recovery_exec L_abs _ _ _ _ p1_abs _ _,
+     H0: recovery_exec L_abs _ _ _ _ _ _ _,
+     H1: SelfSimulation _ _ _ _ _ _ _ _,
      H2: equivalent_states_abs _ _ |- _ ] =>
     eapply_fresh H1 in H;    
     specialize Hx with (3:= H2); edestruct Hx;
@@ -322,8 +325,8 @@ Proof.
   
   (** Show two executions are the same **)
   match goal with
-  | [H: recovery_exec L_abs _ _ _ p2_abs _ _,
-     H0: recovery_exec L_abs _ _ _ p2_abs _ _ |- _ ] =>
+  | [H: recovery_exec L_abs _ _ _ _ p2_abs _ _,
+     H0: recovery_exec L_abs _ _ _ _ p2_abs _ _ |- _ ] =>
     eapply recovery_exec_deterministic_wrt_reboot_state in H;
     eauto; cleanup
   end.
