src/Framework/Simulation/RefinementLift.v
@@ -13,31 +13,31 @@ Section RefinementLift.
     exact (Bind (compile T p2) (fun x => compile T' (p x))).
   Defined.
 
-  Fixpoint oracle_refines_to T (d1: state L_imp) (p: prog L_abs T) get_reboot_state_imp o1 o2 : Prop :=
+  Fixpoint oracle_refines_to T u (d1: state L_imp) (p: prog L_abs T) get_reboot_state_imp o1 o2 : Prop :=
     match p with    
     |Op _ op =>
      exists o2',
      o2 =  [OpToken C_abs o2'] /\
-       CoreRefinement.(token_refines_to) d1 op get_reboot_state_imp o1 o2'
+       CoreRefinement.(token_refines_to) u d1 op get_reboot_state_imp o1 o2'
     | Ret v =>
       (exists d1',
-         exec L_imp o1 d1 (Ret v) (Crashed d1') /\
+         exec L_imp u o1 d1 (Ret v) (Crashed d1') /\
          o2 = [Crash _]) \/
       (exists d1' r,
-         exec L_imp o1 d1 (Ret v) (Finished d1' r) /\
+         exec L_imp u o1 d1 (Ret v) (Finished d1' r) /\
          o2 = [Cont _])
 
     | @Bind _ T1 T2 p1 p2 =>
       exists o1' o1'' o2' o2'',
       o1 = o1'++o1'' /\
       o2 = o2' ++ o2'' /\
-     ((exists d1', exec L_imp o1' d1 (compile T1 p1) (Crashed d1') /\
-         oracle_refines_to T1 d1 p1 get_reboot_state_imp o1' o2') \/
+     ((exists d1', exec L_imp u o1' d1 (compile T1 p1) (Crashed d1') /\
+         oracle_refines_to T1 u d1 p1 get_reboot_state_imp o1' o2') \/
       (exists d1' r ret,
-         exec L_imp o1' d1 (compile T1 p1) (Finished d1' r) /\
-         exec L_imp o1'' d1' (compile T2 (p2 r)) ret /\
-         oracle_refines_to T1 d1 p1 (fun s => s) o1' o2' /\
-         oracle_refines_to T2 d1' (p2 r) get_reboot_state_imp o1'' o2''
+         exec L_imp u o1' d1 (compile T1 p1) (Finished d1' r) /\
+         exec L_imp u o1'' d1' (compile T2 (p2 r)) ret /\
+         oracle_refines_to T1 u d1 p1 (fun s => s) o1' o2' /\
+         oracle_refines_to T2 u d1' (p2 r) get_reboot_state_imp o1'' o2''
          ))
     end.
 
