src/Layers/AbstractLayers/FileDisk/FileDiskLayer.v
@@ -18,7 +18,7 @@ Section FileDisk.
   | DiskFull : token'
   | Cont : token'.
 
-  Definition state' := (user * disk File)%type.
+  Definition state' := (disk File)%type.
   
   Inductive file_disk_prog : Type -> Type :=
   | Read : Inum -> addr -> file_disk_prog (option value)
@@ -30,896 +30,163 @@ Section FileDisk.
   | Recover : file_disk_prog unit.
   
   Inductive exec' :
-    forall T, token' ->  state' -> file_disk_prog T -> @Result state' T -> Prop :=
+    forall T, user -> token' ->  state' -> file_disk_prog T -> @Result state' T -> Prop :=
   | ExecReadSuccess : 
-      forall s inum off file v,
-        let u := fst s in
-        let d := snd s in
+      forall d inum off file v u,
         inum < disk_size ->
         d inum = Some file ->
         file.(owner) = u ->
         nth_error file.(blocks) off = Some v ->
-        exec' Cont s (Read inum off) (Finished s (Some v))
+        exec' u Cont d (Read inum off) (Finished d (Some v))
               
   | ExecReadFail : 
-      forall s inum off file,
-        let u := fst s in
-        let d := snd s in
+      forall d u inum off file,
         (inum >= disk_size \/
          d inum = None \/
-         d inum = Some file /\
-         (file.(owner) <> u \/ nth_error file.(blocks) off = None)) ->
-        exec' Cont s (Read inum off) (Finished s None)
+         (d inum = Some file /\
+         (file.(owner) <> u \/ nth_error file.(blocks) off = None))) ->
+        exec' u Cont d (Read inum off) (Finished d None)
               
   | ExecWriteSuccess :
-      forall s inum file off v,
-        let u := fst s in
-        let d := snd s in
+      forall d u inum file off v,
         inum < disk_size ->
         d inum = Some file ->
         file.(owner) = u ->
         off < length (file.(blocks)) ->
         let new_file := Build_File file.(owner) (updN file.(blocks) off v) in
-        exec' Cont s (Write inum off v) (Finished (u, (upd d inum new_file)) (Some tt))
+        exec' u Cont d (Write inum off v) (Finished (upd d inum new_file) (Some tt))
 
   | ExecWriteFail :
-      forall s inum file off v,
-        let u := fst s in
-        let d := snd s in
+      forall d u inum file off v,
         (inum >= disk_size \/
          d inum = None \/
          d inum = Some file /\
          (file.(owner) <> u \/ off >= length (file.(blocks)))) ->
-        exec' Cont s (Write inum off v) (Finished s None)
+        exec' u Cont d (Write inum off v) (Finished d None)
 
   | ExecExtendSuccess :
-      forall s inum file v,
-        let u := fst s in
-        let d := snd s in
+      forall d u inum file v,
         inum < disk_size ->
         d inum = Some file ->
         file.(owner) = u ->
         let new_file := Build_File file.(owner) (file.(blocks) ++ [v]) in
-        exec' Cont s (Extend inum v) (Finished (u, (upd d inum new_file)) (Some tt))
+        exec' u Cont d (Extend inum v) (Finished (upd d inum new_file) (Some tt))
 
   | ExecExtendFail :
-      forall s inum file v,
-        let u := fst s in
-        let d := snd s in
+      forall d u inum file v,
         (inum >= disk_size \/
          d inum = None \/
          (d inum = Some file /\ file.(owner) <> u)) ->
-        exec' Cont s (Extend inum v) (Finished s None)
+        exec' u Cont d (Extend inum v) (Finished d None)
               
   | ExecExtendFailDiskFull :
-      forall s inum file v,
-        let u := fst s in
-        let d := snd s in
+      forall d u inum file v,
         inum < disk_size ->
         d inum = Some file ->
         file.(owner) = u ->
-        exec' DiskFull s (Extend inum v) (Finished s None)
+        exec' u DiskFull d (Extend inum v) (Finished d None)
 
   | ExecSetOwnerSuccess :
-      forall s inum file o,
-        let u := fst s in
-        let d := snd s in
+      forall d u inum file o,
         inum < disk_size ->
         d inum = Some file ->
         file.(owner) = u ->
         let new_file := Build_File o file.(blocks) in
-        exec' Cont s (SetOwner inum o) (Finished (u, (upd d inum new_file)) (Some tt))
+        exec' u Cont d (SetOwner inum o) (Finished (upd d inum new_file) (Some tt))
 
   | ExecSetOwnerFail :
-      forall s inum file o,
-        let u := fst s in
-        let d := snd s in
+      forall d u inum file o,
         (inum >= disk_size \/
          d inum = None \/
          (d inum = Some file /\ file.(owner) <> u)) ->
-        exec' Cont s (SetOwner inum o) (Finished s None)
+        exec' u Cont d (SetOwner inum o) (Finished d None)
 
   | ExecCreateSuccess :
-      forall s inum owner,
-        let u := fst s in
-        let d := snd s in
+      forall d u inum owner,
         inum < disk_size ->
         d inum = None ->
         let new_file := Build_File owner [] in
-        exec' (NewInum inum) s (Create owner) (Finished (u, (upd d inum new_file)) (Some inum))
+        exec' u (NewInum inum) d (Create owner) (Finished (upd d inum new_file) (Some inum))
 
   | ExecCreateFail :
-      forall s owner,
-        let u := fst s in
-        let d := snd s in
+      forall d u owner,
         (forall inum, inum < disk_size -> d inum <> None) ->
-        exec' InodesFull s (Create owner) (Finished s None)
+        exec' u InodesFull d (Create owner) (Finished d None)
               
   | ExecDeleteSuccess :
-      forall s inum file,
-        let u := fst s in
-        let d := snd s in
+      forall d u inum file,
         inum < disk_size ->
         d inum = Some file ->
         file.(owner) = u ->
-        exec' Cont s (Delete inum) (Finished (u, (Mem.delete d inum)) (Some tt))
+        exec' u Cont d (Delete inum) (Finished (Mem.delete d inum) (Some tt))
 
   | ExecDeleteFail :
-      forall s file inum,
-        let u := fst s in
-        let d := snd s in
+      forall d u file inum,
         (inum >= disk_size \/
          d inum = None \/
          (d inum = Some file /\ file.(owner) <> u)) ->
-        exec' Cont s (Delete inum) (Finished s None)
+        exec' u Cont d (Delete inum) (Finished d None)
 
   | ExecRecover : 
-      forall s,
-        exec' Cont s Recover (Finished s tt)
+      forall d u,
+        exec' u Cont d Recover (Finished d tt)
 
   | ExecCrashBefore :
-      forall d T (p: file_disk_prog T),
-        exec' CrashBefore d p (Crashed d)
+      forall u d T (p: file_disk_prog T),
+        exec' u CrashBefore d p (Crashed d)
 
   | ExecSetOwnerCrashAfter :
-      forall s inum file o,
-        let u := fst s in
-        let d := snd s in
+      forall d u inum file o,
         inum < disk_size ->
         d inum = Some file ->
         file.(owner) = u ->
         let new_file := Build_File o file.(blocks) in
-        exec' CrashAfter s (SetOwner inum o) (Crashed (u, (upd d inum new_file)))
+        exec' u CrashAfter d (SetOwner inum o) (Crashed (upd d inum new_file))
 
   | ExecWriteCrashAfter :
-      forall s inum file off v,
-        let u := fst s in
-        let d := snd s in
+      forall d u inum file off v,
         inum < disk_size ->
         d inum = Some file ->
         file.(owner) = u ->
         off < length (file.(blocks)) ->
         let new_file := Build_File file.(owner) (updN file.(blocks) off v) in
-        exec' CrashAfter s (Write inum off v) (Crashed (u, (upd d inum new_file)))
+        exec' u CrashAfter d (Write inum off v) (Crashed (upd d inum new_file))
 
   | ExecExtendCrashAfter :
-      forall s inum file v,
-        let u := fst s in
-        let d := snd s in
+      forall d u inum file v,
         inum < disk_size ->
         d inum = Some file ->
         file.(owner) = u ->
         let new_file := Build_File file.(owner) (file.(blocks) ++ [v]) in
-        exec' CrashAfter s (Extend inum v) (Crashed (u, (upd d inum new_file)))
+        exec' u CrashAfter d (Extend inum v) (Crashed (upd d inum new_file))
 
   | ExecDeleteCrashAfter :
-      forall s inum file,
-        let u := fst s in
-        let d := snd s in
+      forall d u inum file,
         inum < disk_size ->
         d inum = Some file ->
         file.(owner) = u ->
-        exec' CrashAfter s (Delete inum) (Crashed (u, (Mem.delete d inum)))
+        exec' u CrashAfter d (Delete inum) (Crashed (Mem.delete d inum))
 
   | ExecCreateCrashAfter :
-      forall s inum owner,
-        let u := fst s in
-        let d := snd s in
+      forall d u inum owner,
         inum < disk_size ->
         d inum = None ->
         let new_file := Build_File owner [] in
-        exec' (CrashAfterCreate inum) s (Create owner) (Crashed (u, (upd d inum new_file))).
+        exec' u (CrashAfterCreate inum) d (Create owner) (Crashed (upd d inum new_file)).
 
   Hint Constructors exec' : core.
 
-  Definition weakest_precondition' T (p: file_disk_prog T) :=
-    match p in file_disk_prog T' return (T' -> state' -> Prop) -> token' -> state' -> Prop with
-    | Read inum a =>
-      fun Q o s =>
-        let u := fst s in
-        let d := snd s in
-        (
-          o = Cont /\
-          inum < disk_size /\
-          exists file v,
-            d inum = Some file /\
-            nth_error file.(blocks) a = Some v /\
-            file.(owner) = u /\
-            Q (Some v) s
-        ) \/
-        (
-          o = Cont /\
-          (inum >= disk_size \/
-           d inum = None \/
-           (exists file,
-              d inum = Some file /\
-              (
-                file.(owner) <> u \/
-                nth_error file.(blocks) a = None
-              )
-           )
-          ) /\
-          Q None s
-        )
-          
-    | Write inum a v =>
-      fun Q o s =>
-        let u := fst s in
-        let d := snd s in
-        (
-          o = Cont /\
-          inum < disk_size /\  
-          exists file,
-            d inum = Some file /\
-            file.(owner) = u /\
-            a < length (file.(blocks)) /\
-            let new_file :=
-                Build_File file.(owner) (updN file.(blocks) a v) in
-            Q (Some tt) (u, upd d inum new_file)
-        ) \/
-        (
-          o = Cont /\
-          (inum >= disk_size \/
-           d inum = None \/
-           (exists file,
-              d inum = Some file /\
-              (
-                file.(owner) <> u \/
-                a >= length (file.(blocks))
-              )
-           )
-          ) /\
-          Q None s
-        )
-          
-    | SetOwner inum u' =>
-      fun Q o s =>
-        let u := fst s in
-        let d := snd s in
-        (
-          o = Cont /\
-          inum < disk_size /\
-          exists file,
-            let new_file := Build_File u' file.(blocks) in
-            d inum = Some file /\
-            file.(owner) = u /\
-            Q (Some tt) (u, upd d inum new_file)
-        ) \/
-        (
-          o = Cont /\
-          (inum >= disk_size \/ d inum = None \/
-           exists file,
-             d inum = Some file /\
-             file.(owner) <> u) /\
-          Q None s
-        )
-          
-    | Create u' =>
-      fun Q o s =>
-        let u := fst s in
-        let d := snd s in
-        (
-          o = InodesFull /\
-          (forall inum, inum < disk_size -> d inum <> None) /\
-          Q None s
-        ) \/
-
-        (exists inum,
-           o = NewInum inum /\
-           inum < disk_size /\ 
-           d inum = None /\
-           let new_file := Build_File u' [] in
-           Q (Some inum) (u, upd d inum new_file)
-        )
-          
-    | Delete inum =>
-      fun Q o s =>
-        let u := fst s in
-        let d := snd s in
-        (
-          o = Cont /\
-          inum < disk_size /\
-          (exists file,
-             d inum = Some file /\ 
-             file.(owner) = u) /\
-          Q (Some tt) (u, Mem.delete d inum)
-        ) \/
-        (
-          o = Cont /\
-          (inum >= disk_size \/
-           d inum = None \/
-           exists file,
-             d inum = Some file /\
-             file.(owner) <> u) /\
-          Q None s
-        )
-    | Extend inum v =>
-      fun Q o s =>
-        let u := fst s in
-        let d := snd s in
-        (
-          o = DiskFull /\
-          inum < disk_size /\
-          (exists file,
-             d inum = Some file /\ 
-             file.(owner) = u) /\
-          Q None s
-        ) \/
-        (
-          o = Cont /\
-          inum < disk_size /\
-          exists file,
-            d inum = Some file /\
-            file.(owner) = u /\
-            let new_file := Build_File file.(owner) (file.(blocks) ++ [v]) in
-            Q (Some tt) (u, upd d inum new_file)
-        ) \/
-        (
-          o = Cont /\
-          (inum >= disk_size \/ d inum = None \/
-           exists file,
-             d inum = Some file /\
-             file.(owner) <> u) /\
-          Q None s
-        )
-    | Recover =>
-      fun Q o s =>
-        o = Cont /\
-        Q tt s
-    end.
-
-  
-  Definition weakest_crash_precondition' T (p: file_disk_prog T) :=
-    match p in file_disk_prog T' return (state' -> Prop) -> token' -> state' -> Prop with
-    | Read inum a =>
-      fun Q o s =>
-        let u := fst s in
-        let d := snd s in
-        (
-          o = CrashBefore /\
-          Q s
-        )
-          
-    | Write inum a v =>
-      fun Q o s =>
-        let u := fst s in
-        let d := snd s in
-        (
-          o = CrashBefore /\
-          Q s
-        ) \/
-        (
-          o = CrashAfter /\
-          inum < disk_size /\  
-          exists file,
-            d inum = Some file /\
-            file.(owner) = u /\
-            a < length (file.(blocks)) /\
-            let new_file :=
-                Build_File file.(owner) (updN file.(blocks) a v) in
-            Q (u, upd d inum new_file)
-        )
-          
-    | SetOwner inum u' =>
-      fun Q o s =>
-        let u := fst s in
-        let d := snd s in
-        (
-          o = CrashBefore /\
-          Q s
-        ) \/
-        (
-          o = CrashAfter /\
-          inum < disk_size /\
-          exists file,
-            let new_file := Build_File u' file.(blocks) in
-            d inum = Some file /\
-            file.(owner) = u /\
-            Q (u, upd d inum new_file)
-        )
-          
-    | Create u' =>
-      fun Q o s =>
-        let u := fst s in
-        let d := snd s in
-        (
-          o = CrashBefore /\
-          Q s
-        ) \/
-        (exists inum,
-           o = CrashAfterCreate inum /\
-           inum < disk_size /\ 
-           d inum = None /\
-           let new_file := Build_File u' [] in
-           Q (u, upd d inum new_file)
-        )
-          
-    | Delete inum =>
-      fun Q o s =>
-        let u := fst s in
-        let d := snd s in
-        (
-          o = CrashBefore /\
-          Q s
-        ) \/
-        (
-          o = CrashAfter /\
-          inum < disk_size /\
-          (exists file,
-             d inum = Some file /\
-             file.(owner) = u) /\
-          Q (u, Mem.delete d inum)
-        )
-          
-    | Extend inum v =>
-      fun Q o s =>
-        let u := fst s in
-        let d := snd s in
-        (
-          o = CrashBefore /\
-          Q s
-        ) \/
-        (
-          o = CrashAfter /\
-          inum < disk_size /\
-          exists file,
-            d inum = Some file /\
-            file.(owner) = u /\
-            let new_file := Build_File file.(owner) (file.(blocks) ++ [v]) in
-            Q (u, upd d inum new_file)
-        )
-    | Recover =>
-      fun Q o s =>
-        o = CrashBefore /\
-        Q s
-    end.
-
-  Definition strongest_postcondition' T (p: file_disk_prog T) :=
-    match p in file_disk_prog T' return (token' -> state' -> Prop) -> T' -> state' -> Prop with
-    | Read inum a =>
-      fun P t s' =>
-        (
-          exists s,
-            let u := fst s in
-            let d := snd s in
-            P Cont s /\
-            inum < disk_size /\
-            exists file v,
-              d inum = Some file /\
-              file.(owner) = u /\
-              nth_error file.(blocks) a = Some v /\
-              t = Some v /\
-              s' = s
-        ) \/
-        (
-          exists s,
-            let u := fst s in
-            let d := snd s in
-            P Cont s /\
-            (inum >= disk_size \/
-             d inum = None \/
-             (exists file,
-                d inum = Some file /\
-                (
-                  file.(owner) <> u \/
-                  nth_error file.(blocks) a = None
-                )
-             )
-            ) /\
-            t = None /\
-            s' = s
-        )
-          
-    | Write inum a v =>
-      fun P t s' =>
-        (
-          exists s,
-            let u := fst s in
-            let d := snd s in
-            P Cont s /\
-            inum < disk_size /\  
-            exists file,
-              d inum = Some file /\
-              file.(owner) = u /\
-              a < length (file.(blocks)) /\
-              let new_file :=
-                  Build_File file.(owner) (updN file.(blocks) a v) in
-              t = (Some tt) /\
-              s' = (u, upd d inum new_file)
-        ) \/
-        (
-          exists s,
-            let u := fst s in
-            let d := snd s in
-            P Cont s /\
-            (inum >= disk_size \/
-             d inum = None \/
-             (exists file,
-                d inum = Some file /\
-                (
-                  file.(owner) <> u \/
-                  a >= length (file.(blocks))
-                )
-             )
-            ) /\
-            t = None /\
-            s' = s
-        )
-          
-    | SetOwner inum u' =>
-      fun P t s' =>
-        (exists s,
-           let u := fst s in
-           let d := snd s in
-           P Cont s /\
-           inum < disk_size /\
-           exists file,
-             let new_file := Build_File u' file.(blocks) in
-             d inum = Some file /\
-             file.(owner) = u /\
-             t = (Some tt) /\
-             s' = (u, upd d inum new_file)
-        ) \/
-        (exists s,
-           let u := fst s in
-           let d := snd s in
-           P Cont s /\
-           (inum >= disk_size \/
-            d inum = None \/
-            exists file,
-              d inum = Some file /\
-              file.(owner) <> u) /\
-           t = None /\
-           s' = s
-        )
-          
-    | Create u' =>
-      fun P t s' =>
-        (exists s,
-           let u := fst s in
-           let d := snd s in
-           P InodesFull s /\
-           (forall inum, inum < disk_size -> d inum <> None) /\
-           t = None /\
-           s' = s
-        ) \/
-        (exists s inum,
-           let u := fst s in
-           let d := snd s in
-           P (NewInum inum) s /\
-           inum < disk_size /\ 
-           d inum = None /\
-           let new_file := Build_File u' [] in
-           t = (Some inum) /\
-           s' = (u, upd d inum new_file)
-        )
-          
-    | Delete inum =>
-      fun P t s' =>
-        (
-          exists s,
-            let u := fst s in
-            let d := snd s in
-            P Cont s /\
-            inum < disk_size /\
-            (exists file,
-               d inum = Some file /\
-               file.(owner) = u
-            ) /\
-            t = (Some tt) /\
-            s' = (u, Mem.delete d inum)
-        ) \/
-        (exists s,
-           let u := fst s in
-           let d := snd s in
-           P Cont s /\
-           (inum >= disk_size \/
-            d inum = None \/
-            exists file,
-              d inum = Some file /\
-              file.(owner) <> u) /\
-           t = None /\
-           s' = s
-        )
-          
-    | Extend inum v =>
-      fun P t s' =>
-        (exists s,
-           let u := fst s in
-           let d := snd s in
-           P DiskFull s /\
-           inum < disk_size /\
-           (exists file,
-              d inum = Some file /\
-              file.(owner) = u) /\
-           t = None /\
-           s' = s
-        ) \/
-        (exists s,
-           let u := fst s in
-           let d := snd s in
-           P Cont s /\
-           inum < disk_size /\
-           exists file,
-             d inum = Some file /\
-             file.(owner) = u /\
-             let new_file := Build_File file.(owner) (file.(blocks) ++ [v]) in
-             t = (Some tt) /\
-             s' = (u, upd d inum new_file)
-        ) \/
-        (exists s,
-           let u := fst s in
-           let d := snd s in
-           P Cont s /\
-           (inum >= disk_size \/
-            d inum = None \/
-            exists file,
-              d inum = Some file /\
-              file.(owner) <> u) /\
-           t = None /\
-           s' = s
-        )
-    | Recover =>
-      fun P t s' =>
-          exists s,
-            P Cont s /\
-            t = tt /\
-            s' = s
-    end.
-  
-  Definition strongest_crash_postcondition' T (p: file_disk_prog T) :=
-    match p in file_disk_prog T' return (token' -> state' -> Prop) -> state' -> Prop with
-    | Read inum a =>
-      fun P s' =>
-        (exists s,
-           P CrashBefore s /\
-           s' = s
-        )
-          
-    | Write inum a v =>
-      fun P s' =>
-        (exists s,
-           P CrashBefore s /\
-           s' = s
-        ) \/
-        (exists s,
-           let u := fst s in
-           let d := snd s in
-           P CrashAfter s /\
-           inum < disk_size /\  
-           exists file,
-             d inum = Some file /\
-             file.(owner) = u /\
-             a < length (file.(blocks)) /\
-             let new_file :=
-                 Build_File file.(owner) (updN file.(blocks) a v) in
-             s' = (u, upd d inum new_file)
-        )
-          
-    | SetOwner inum u' =>
-      fun P s' =>
-        (exists s,
-           P CrashBefore s /\
-           s' = s
-        ) \/
-        (exists s,
-           let u := fst s in
-           let d := snd s in
-           P CrashAfter s /\
-           inum < disk_size /\
-           exists file,
-             let new_file := Build_File u' file.(blocks) in
-             d inum = Some file /\
-             file.(owner) = u /\
-             s' = (u, upd d inum new_file)
-        )
-          
-    | Create u' =>
-      fun P s' =>
-        (exists s,
-           P CrashBefore s /\
-           s' = s
-        ) \/
-        (exists s inum,
-           let u := fst s in
-           let d := snd s in
-           P (CrashAfterCreate inum) s /\
-           inum < disk_size /\ 
-           d inum = None /\
-           let new_file := Build_File u' [] in
-           s' = (u, upd d inum new_file)
-        )
-          
-    | Delete inum =>
-      fun P s' =>
-        (exists s,
-           P CrashBefore s /\
-           s' = s
-        ) \/
-        (exists s,
-           let u := fst s in
-           let d := snd s in
-           P CrashAfter s /\
-           inum < disk_size /\
-           (exists file,
-              d inum = Some file /\
-             file.(owner) = u) /\
-           s' = (u, Mem.delete d inum)
-        )
-    | Extend inum v =>
-      fun P s' =>
-        (exists s,
-           P CrashBefore s /\
-           s' = s
-        ) \/
-        (exists s,
-           let u := fst s in
-           let d := snd s in
-           P CrashAfter s /\
-           inum < disk_size /\
-           exists file,
-             d inum = Some file /\
-             file.(owner) = u /\
-             let new_file := Build_File file.(owner) (file.(blocks) ++ [v]) in
-             s' = (u, upd d inum new_file)
-        )
-
-    | Recover =>
-      fun P s' =>
-        exists s,
-           P CrashBefore s /\
-           s' = s
-    end.
-
-  Arguments skipn : simpl never.
-  Theorem sp_complete':
-    forall T (p: file_disk_prog T) P (Q: _ -> _ -> Prop),
-      (forall t s', strongest_postcondition' p P t s' -> Q t s') <->
-      (forall o s s' t, P o s -> exec' o s p (Finished s' t) -> Q t s').
-  Proof.
-    intros; destruct p; simpl; eauto;
-    split; intros;
-    repeat (split_ors; cleanup; eauto);
-    eapply H; eauto;
-    try match goal with
-        | [H: exec' _ _ _ _ |- _] =>
-          inversion H; clear H; cleanup
-        end;
-    try solve [left; eexists; intuition eauto;               
-               repeat eexists; intuition eauto; cleanup; simpl; eauto ];
-    try solve [right; repeat eexists; intuition eauto ];
-    try solve [intuition eauto;
-               repeat eexists; intuition eauto;
-               try solve [ econstructor; eauto ];
-               simpl; cleanup; eauto ];
-    rewrite <- H3 at 2; eauto.
-    
-    Unshelve.
-    all: repeat econstructor; eauto.
-    all: exact user0.
-  Qed.
-
-  Theorem scp_complete':
-    forall T (p: file_disk_prog T) P (Q:  _ -> Prop),
-      (forall s', strongest_crash_postcondition' p P s' -> Q s') <->
-      (forall o s s', P o s -> exec' o s p (Crashed s') -> Q s').
-  Proof.
-    intros; destruct p; simpl; eauto;
-    split; intros;
-    repeat (split_ors; cleanup);
-    eapply H; eauto;
-    repeat
-      match goal with
-      | [H: exec' _ _ _ _ |- _] =>
-        inversion H; clear H; cleanup
-      end;
-    try solve [left; eexists; intuition eauto;               
-               repeat eexists; intuition eauto; cleanup; simpl; eauto ];
-    try solve [right; repeat eexists; intuition eauto ];
-    try solve [intuition eauto;
-               repeat eexists; intuition eauto;
-               try solve [
-                     econstructor;
-                     [| try solve [
-                              try rewrite <- H3 at 2;
-                              econstructor;  eauto
-                            ]
-                     ]; eauto
-                   ];
-               simpl; cleanup; eauto
-              ].
-
-    try rewrite <- H3 at 2;
-    econstructor;  eauto.
-    try rewrite <- H3 at 2;
-    econstructor;  eauto.
-    
-    Unshelve.
-    all: repeat econstructor; eauto.
-    all: exact user0.
-  Qed.
-  
-    Theorem wp_complete':
-    forall T (p: file_disk_prog T) H Q,
-      (forall o s, H o s -> weakest_precondition' p Q o s) <->
-      (forall o s, H o s -> (exists s' v, exec' o s p (Finished s' v) /\ Q v s')).
-  Proof.
-    intros; destruct p; simpl; eauto;
-    split; intros;
-    specialize H0 with (1:= X);
-    cleanup; eauto;
-    try match goal with
-        | [H: exec' _ _ _ _ |- _] =>
-          inversion H; clear H; cleanup
-        end;
-    try solve [
-          repeat (split_ors; cleanup; eauto);
-          do 2 eexists; intuition eauto;
-          try solve [ econstructor; eauto ];
-          simpl; cleanup; eauto ];
-    try solve [
-          left; intuition eauto;
-          do 2 eexists; intuition eauto;
-          try solve [ econstructor; eauto ];
-          simpl; cleanup; eauto ];
-    try solve [
-          right;intuition eauto;
-          do 2 eexists; intuition eauto;
-          try solve [ econstructor; eauto ];
-          simpl; cleanup; eauto ].
-    
-    Unshelve.
-    all: repeat econstructor; eauto.
-    all: exact user0.
-  Qed.
-  
-  Theorem wcp_complete':
-    forall T (p: file_disk_prog T) H C,
-      (forall o s, H o s -> weakest_crash_precondition' p C o s) <->
-      (forall o s, H o s -> (exists s', exec' o s p (Crashed s') /\ C s')).
-  Proof.
-    unfold weakest_crash_precondition';
-    intros; destruct p; simpl; eauto;
-    split; intros;
-    specialize H0 with (1:= X);
-    cleanup; eauto;
-    try repeat
-        match goal with
-        | [H: exec' _ _ _ _ |- _] =>
-          inversion H; clear H; cleanup
-        end;
-
-    try solve [
-          repeat (split_ors; cleanup; eauto);
-          repeat eexists; intuition eauto;
-          try solve [ repeat econstructor; eauto; congruence ];
-          try congruence; simpl; cleanup; eauto ];
-    try solve [
-          left; intuition eauto;
-          repeat eexists; intuition eauto;
-          try solve [ econstructor; eauto ];
-          simpl; cleanup; eauto ];
-    try solve [
-          right;intuition eauto;
-          repeat eexists; intuition eauto;
-          try solve [ econstructor; eauto ];
-          simpl; cleanup; eauto ].
-    
-    Unshelve.
-    all: repeat econstructor; eauto.
-    all: exact user0.
-  Qed.
 
   Theorem exec_deterministic_wrt_token' :
-    forall o s T (p: file_disk_prog T) ret1 ret2,
-      exec' o s p ret1 ->
-      exec' o s p ret2 ->
+    forall u o s T (p: file_disk_prog T) ret1 ret2,
+      exec' u o s p ret1 ->
+      exec' u o s p ret2 ->
       ret1 = ret2.
   Proof.
     intros; destruct p; simpl in *; cleanup;
     repeat
       match goal with
-      | [H: exec' _ _ _ _ |- _] =>
+      | [H: exec' _ _ _ _ _ |- _] =>
         inversion H; clear H; try split_ors; cleanup
       end;
     try solve [ repeat (cleanup; intuition eauto; try congruence; try lia) ].
@@ -929,16 +196,6 @@ Section FileDisk.
     Build_Core
       file_disk_prog
       exec'
-      (*
-        weakest_precondition'
-      weakest_crash_precondition'
-      strongest_postcondition'
-      strongest_crash_postcondition'
-      wp_complete'
-      wcp_complete'
-      sp_complete'
-      scp_complete'
-       *)
       exec_deterministic_wrt_token'.
 
   Definition FileDiskLang := Build_Language FileDiskOperation.
