src/Layers/BasicLayers/Cache/CacheLayer.v
@@ -21,127 +21,35 @@ Section CacheLayer.
   | Flush : cache_prog unit.
   
   Inductive exec' :
-    forall T, token' ->  state' -> cache_prog T -> @Result state' T -> Prop :=
+    forall T, user -> token' ->  state' -> cache_prog T -> @Result state' T -> Prop :=
   | ExecRead : 
-      forall d a,
-        exec' Cont d (Read a) (Finished d (d a))
+      forall d a u,
+        exec' u Cont d (Read a) (Finished d (d a))
              
   | ExecWrite :
-      forall d a v,
-        exec' Cont d (Write a v) (Finished (upd d a v) tt)
+      forall d a v u,
+        exec' u Cont d (Write a v) (Finished (upd d a v) tt)
 
   | ExecFlush :
-      forall d,
-        exec' Cont d Flush (Finished empty_mem tt)
+      forall d u,
+        exec' u Cont d Flush (Finished empty_mem tt)
               
   | ExecCrash :
-      forall T d (p: cache_prog T),
-        exec' Crash d p (Crashed d).
+      forall T d (p: cache_prog T) u,
+        exec' u Crash d p (Crashed d).
 
   Hint Constructors exec' : core.
-  
-  Definition weakest_precondition' T (p: cache_prog T) :=
-   match p in cache_prog T' return (T' -> state' -> Prop) -> token' -> state' -> Prop with
-   | Read a =>
-    fun Q o s =>
-        o = Cont /\
-        Q (s a) s
-   | Write a v =>
-     fun Q o s =>
-        o = Cont /\
-        Q tt (upd s a v)
-   | Flush =>
-     fun Q o s =>
-        o = Cont /\
-        Q tt empty_mem
-   end.
-
-  Definition weakest_crash_precondition' T (p: cache_prog T) :=
-    fun (Q: state' -> Prop) o (s: state') => o = Crash /\ Q s.
-
-  Definition strongest_postcondition' T (p: cache_prog T) :=
-   match p in cache_prog T' return (token' -> state' -> Prop) -> T' -> state' -> Prop with
-   | Read a =>
-     fun P t s' =>
-       exists s,
-        P Cont s /\
-        t = s a /\
-        s' = s
-   | Write a v =>
-     fun P t s' =>
-       exists s,
-         P Cont s /\
-         t = tt /\
-         s' = upd s a v
-   | Flush  =>
-     fun P t s' =>
-       exists s,
-         P Cont s /\
-         t = tt /\
-         s' = empty_mem
-   end.
-
-  Definition strongest_crash_postcondition' T (p: cache_prog T) :=
-    fun (P: token' -> state' -> Prop) (s: state') => P Crash s.
-
-  Theorem sp_complete':
-    forall T (p: cache_prog T) P (Q: _ -> _ -> Prop),
-      (forall t s', strongest_postcondition' p P t s' -> Q t s') <->
-      (forall o s s' t, P o s -> exec' o s p (Finished s' t) -> Q t s').
-  Proof.
-    intros; destruct p; simpl; eauto;
-    split; intros;
-    try inversion H1; cleanup;
-    eapply H; eauto;
-    do 2 eexists; eauto.    
-  Qed.
-
-  Theorem scp_complete':
-    forall T (p: cache_prog T) P (Q:  _ -> Prop),
-      (forall s', strongest_crash_postcondition' p P s' -> Q s') <->
-      (forall o s s', P o s -> exec' o s p (Crashed s') -> Q s').
-  Proof.
-    intros; destruct p; simpl; eauto;
-    split; intros;
-    try inversion H1; cleanup;
-    eapply H; eauto.
-  Qed.
-  
-  Theorem wp_complete':
-    forall T (p: cache_prog T) H Q,
-      (forall o s, H o s -> weakest_precondition' p Q o s) <->
-      (forall o s, H o s -> (exists s' v, exec' o s p (Finished s' v) /\ Q v s')).
-  Proof.
-    intros; destruct p; simpl; eauto;
-    split; intros;
-    specialize H0 with (1:= X);
-    cleanup; eauto;
-    inversion H0; cleanup; eauto.
-  Qed.
-  
-  Theorem wcp_complete':
-    forall T (p: cache_prog T) H C,
-      (forall o s, H o s -> weakest_crash_precondition' p C o s) <->
-      (forall o s, H o s -> (exists s', exec' o s p (Crashed s') /\ C s')).
-  Proof.
-    unfold weakest_crash_precondition';
-    intros; destruct p; simpl; eauto;
-    split; intros;
-    specialize H0 with (1:= X);
-    cleanup; eauto;
-    inversion H0; cleanup; eauto.
-  Qed.
 
   Theorem exec_deterministic_wrt_token' :
-    forall o s T (p: cache_prog T) ret1 ret2,
-      exec' o s p ret1 ->
-      exec' o s p ret2 ->
+    forall u o s T (p: cache_prog T) ret1 ret2,
+      exec' u o s p ret1 ->
+      exec' u o s p ret2 ->
       ret1 = ret2.
   Proof.
     intros; destruct p; simpl in *; cleanup;
     repeat
       match goal with
-      | [H: exec' _ _ _ _ |- _] =>
+      | [H: exec' _ _ _ _ _ |- _] =>
         inversion H; clear H; cleanup
       end; eauto.
   Qed.
@@ -150,20 +58,8 @@ Section CacheLayer.
     Build_Core
       cache_prog
       exec'
-      (* 
-         weakest_precondition'
-      weakest_crash_precondition'
-      strongest_postcondition'
-      strongest_crash_postcondition'
-      wp_complete'
-      wcp_complete'
-      sp_complete'
-      scp_complete'
-       *)
       exec_deterministic_wrt_token'.
 
   Definition CacheLang := Build_Language CacheOperation.
-
-Notation "p >> s" := (p s) (right associativity, at level 60, only parsing).
 
 End CacheLayer.
