src/Layers/BasicLayers/Storage/StorageLayer.v
@@ -20,131 +20,36 @@ Section StorageLayer.
 
   
   Inductive exec' :
-    forall T, token' ->  state' -> storage_prog T -> @Result state' T -> Prop :=
+    forall T, user -> token' ->  state' -> storage_prog T -> @Result state' T -> Prop :=
   | ExecGet : 
-      forall d v,
+      forall d v u,
         d = Some v ->
-        exec' Cont d Get (Finished d v)
+        exec' u Cont d Get (Finished d v)
              
   | ExecPut :
-      forall d v,
-        exec' Cont d (Put v) (Finished (Some v) tt)
+      forall d v u,
+        exec' u Cont d (Put v) (Finished (Some v) tt)
 
   | ExecDelete :
-      forall d,
-        exec' Cont d Delete (Finished None tt)
+      forall d u,
+        exec' u Cont d Delete (Finished None tt)
               
   | ExecCrash :
-      forall T d (p: storage_prog T),
-        exec' Crash d p (Crashed d).
+      forall T d (p: storage_prog T) u,
+        exec' u Crash d p (Crashed d).
 
   Hint Constructors exec' : core.
   
-  Definition weakest_precondition' T (p: storage_prog T) :=
-   match p in storage_prog T' return (T' -> state' -> Prop) -> token' -> state' -> Prop with
-   | Get =>
-     fun Q o s =>
-       exists v, 
-        o = Cont /\
-        s = Some v /\
-        Q v s
-   | Put v =>
-     fun Q o s =>
-        o = Cont /\
-        Q tt (Some v)
-   | Delete =>
-     fun Q o s =>
-        o = Cont /\
-        Q tt None
-   end.
-
-  Definition weakest_crash_precondition' T (p: storage_prog T) :=
-    fun (Q: state' -> Prop) o (s: state') => o = Crash /\ Q s.
-
-  Definition strongest_postcondition' T (p: storage_prog T) :=
-   match p in storage_prog T' return (token' -> state' -> Prop) -> T' -> state' -> Prop with
-   | Get =>
-     fun P t s' =>
-       exists s v,
-        P Cont s /\
-        s = Some v /\
-        t = v /\
-        s' = s
-   | Put v =>
-     fun P t s' =>
-       exists s,
-         P Cont s /\
-         t = tt /\
-         s' = Some v
-   | Delete  =>
-     fun P t s' =>
-       exists s,
-         P Cont s /\
-         t = tt /\
-         s' = None
-   end.
-
-  Definition strongest_crash_postcondition' T (p: storage_prog T) :=
-    fun (P: token' -> state' -> Prop) (s: state') => P Crash s.
-
-  Theorem sp_complete':
-    forall T (p: storage_prog T) P (Q: _ -> _ -> Prop),
-      (forall t s', strongest_postcondition' p P t s' -> Q t s') <->
-      (forall o s s' t, P o s -> exec' o s p (Finished s' t) -> Q t s').
-  Proof.
-    intros; destruct p; simpl; eauto;
-    split; intros;
-    try inversion H1; cleanup;
-    eapply H; eauto;
-    do 2 eexists; eauto.    
-  Qed.
-
-  Theorem scp_complete':
-    forall T (p: storage_prog T) P (Q:  _ -> Prop),
-      (forall s', strongest_crash_postcondition' p P s' -> Q s') <->
-      (forall o s s', P o s -> exec' o s p (Crashed s') -> Q s').
-  Proof.
-    intros; destruct p; simpl; eauto;
-    split; intros;
-    try inversion H1; cleanup;
-    eapply H; eauto.
-  Qed.
-  
-  Theorem wp_complete':
-    forall T (p: storage_prog T) H Q,
-      (forall o s, H o s -> weakest_precondition' p Q o s) <->
-      (forall o s, H o s -> (exists s' v, exec' o s p (Finished s' v) /\ Q v s')).
-  Proof.
-    intros; destruct p; simpl; eauto;
-    split; intros;
-    specialize H0 with (1:= X);
-    cleanup; eauto;
-    inversion H0; cleanup; eauto.
-  Qed.
-  
-  Theorem wcp_complete':
-    forall T (p: storage_prog T) H C,
-      (forall o s, H o s -> weakest_crash_precondition' p C o s) <->
-      (forall o s, H o s -> (exists s', exec' o s p (Crashed s') /\ C s')).
-  Proof.
-    unfold weakest_crash_precondition';
-    intros; destruct p; simpl; eauto;
-    split; intros;
-    specialize H0 with (1:= X);
-    cleanup; eauto;
-    inversion H0; cleanup; eauto.
-  Qed.
-
   Theorem exec_deterministic_wrt_token' :
-    forall o s T (p: storage_prog T) ret1 ret2,
-      exec' o s p ret1 ->
-      exec' o s p ret2 ->
+    forall u o s T (p: storage_prog T) ret1 ret2,
+      exec' u o s p ret1 ->
+      exec' u o s p ret2 ->
       ret1 = ret2.
   Proof.
     intros; destruct p; simpl in *; cleanup;
     repeat
       match goal with
-      | [H: exec' _ _ _ _ |- _] =>
+      | [H: exec' _ _ _ _ _ |- _] =>
         inversion H; clear H; cleanup
       end; eauto.
   Qed.
@@ -153,20 +58,8 @@ Section StorageLayer.
     Build_Core
       storage_prog
       exec'
-      (*
-        weakest_precondition'
-      weakest_crash_precondition'
-      strongest_postcondition'
-      strongest_crash_postcondition'
-      wp_complete'
-      wcp_complete'
-      sp_complete'
-      scp_complete'
-      *)
       exec_deterministic_wrt_token'.
 
   Definition StorageLang := Build_Language StorageOperation.
-
-  Notation "p >> s" := (p s) (right associativity, at level 60, only parsing).
   
 End StorageLayer.
