src/Framework/Layer/Automation.v
@@ -6,21 +6,21 @@ Ltac invert_exec'' H :=
 
   
 Lemma bind_sep:
-  forall O (L: Language O) T T' o d (p1: prog L T) (p2: T -> prog L T') ret,
-    exec L o d (Bind p1 p2) ret ->
+  forall O (L: Language O) T T' u o d (p1: prog L T) (p2: T -> prog L T') ret,
+    exec L u o d (Bind p1 p2) ret ->
     match ret with
     | Finished d' r =>
     (exists o1 o2 d1 r1,
-       exec L o1 d p1 (Finished d1 r1) /\
-       exec L o2 d1 (p2 r1) ret /\
+       exec L u o1 d p1 (Finished d1 r1) /\
+       exec L u o2 d1 (p2 r1) ret /\
        o = o1++o2)
   | Crashed d' =>
     (exists o1 o2,
     o = o1++o2 /\    
-    (exec L o1 d p1 (Crashed d') \/
+    (exec L u o1 d p1 (Crashed d') \/
      (exists d1 r1,
-        exec L o1 d p1 (Finished d1 r1) /\
-        exec L o2 d1 (p2 r1) ret)))
+        exec L u o1 d p1 (Finished d1 r1) /\
+        exec L u o2 d1 (p2 r1) ret)))
     end.
 Proof.
   intros.
@@ -32,8 +32,8 @@ Proof.
 
  Local Lemma lift1_invert_exec :
     forall O1 O2 (L1: Language O1) (Lc: Language (HorizontalComposition O1 O2))
-      T (p1: L1.(prog) T) (o: Lc.(oracle)) s s' t,
-      exec Lc o s (lift_L1 O2 p1) (Finished s' t) ->
+      T (p1: L1.(prog) T) (o: Lc.(oracle)) u s s' t,
+      exec Lc u o s (lift_L1 O2 p1) (Finished s' t) ->
       exists o1,
         o = map (fun o =>
                    match o with
@@ -46,12 +46,12 @@ Proof.
                     Language.Crash _
                    end) o1 /\
         snd s = snd s' /\
-        exec L1 o1 (fst s) p1 (Finished (fst s') t).
+        exec L1 u o1 (fst s) p1 (Finished (fst s') t).
   Proof.
     induction p1; simpl; intros.
     {      
       invert_exec'' H.
-      invert_exec'' H5.      
+      invert_exec'' H6.      
       eexists; intuition eauto.
       simpl; eauto.
     }
@@ -75,8 +75,8 @@ Proof.
     
 Local Lemma lift2_invert_exec :
     forall O1 O2 (L2: Language O2) (Lc: Language (HorizontalComposition O1 O2))
-      T (p2: L2.(prog) T) (o: Lc.(oracle)) s s' t,
-      exec Lc o s (lift_L2 O1 p2) (Finished s' t) ->
+      T (p2: L2.(prog) T) (o: Lc.(oracle)) u s s' t,
+      exec Lc u o s (lift_L2 O1 p2) (Finished s' t) ->
       exists o2,
         o = map (fun o =>
                    match o with
@@ -89,12 +89,12 @@ Local Lemma lift2_invert_exec :
                     Language.Crash _
                    end) o2 /\
         fst s = fst s' /\
-        exec L2 o2 (snd s) p2 (Finished (snd s') t).
+        exec L2 u o2 (snd s) p2 (Finished (snd s') t).
   Proof.
     induction p2; simpl; intros.
     {
       invert_exec'' H.
-      invert_exec'' H5.
+      invert_exec'' H6.
       eexists; intuition eauto.
       simpl; eauto.
     }
@@ -117,8 +117,8 @@ Local Lemma lift2_invert_exec :
 
   Local Lemma lift1_invert_exec_crashed :
     forall O1 O2 (L1: Language O1) (Lc: Language (HorizontalComposition O1 O2))
-      T (p1: L1.(prog) T) (o: Lc.(oracle)) s s',
-      exec Lc o s (lift_L1 O2 p1) (Crashed s') ->
+      T (p1: L1.(prog) T) (o: Lc.(oracle)) u s s',
+      exec Lc u o s (lift_L1 O2 p1) (Crashed s') ->
       exists o1 o2,
         o = map (fun o =>
                    match o with
@@ -131,12 +131,12 @@ Local Lemma lift2_invert_exec :
                     Language.Crash _
                    end) o1 ++ o2 /\
         snd s = snd s' /\
-        exec L1 o1 (fst s) p1 (Crashed (fst s')).
+        exec L1 u o1 (fst s) p1 (Crashed (fst s')).
   Proof.
     induction p1; simpl; intros.
     {      
       invert_exec'' H.
-      invert_exec'' H5.      
+      invert_exec'' H6.      
       do 2 eexists; intuition eauto.
       2: simpl; constructor; eauto.
       simpl; eauto.
@@ -149,7 +149,7 @@ Local Lemma lift2_invert_exec :
     }
     {
       invert_exec'' H0.
-      eapply lift1_invert_exec in H6; cleanup.
+      eapply lift1_invert_exec in H7; cleanup.
       edestruct H; eauto; cleanup.
       
       do 2 eexists; split.
@@ -171,8 +171,8 @@ Local Lemma lift2_invert_exec :
     
 Local Lemma lift2_invert_exec_crashed :
     forall O1 O2 (L2: Language O2) (Lc: Language (HorizontalComposition O1 O2))
-      T (p2: L2.(prog) T) (o: Lc.(oracle)) s s',
-      exec Lc o s (lift_L2 O1 p2) (Crashed s') ->
+      T (p2: L2.(prog) T) (o: Lc.(oracle)) u s s',
+      exec Lc u o s (lift_L2 O1 p2) (Crashed s') ->
       exists o' o2,
         o = map (fun o =>
                    match o with
@@ -185,12 +185,12 @@ Local Lemma lift2_invert_exec_crashed :
                     Language.Crash _
                    end) o2 ++ o' /\
         fst s = fst s' /\
-        exec L2 o2 (snd s) p2 (Crashed (snd s')).
+        exec L2 u o2 (snd s) p2 (Crashed (snd s')).
   Proof.
     induction p2; simpl; intros.
     {      
       invert_exec'' H.
-      invert_exec'' H5.      
+      invert_exec'' H6.      
       do 2 eexists; intuition eauto.
       2: simpl; constructor; eauto.
       simpl; eauto.
@@ -203,7 +203,7 @@ Local Lemma lift2_invert_exec_crashed :
     }
     {
       invert_exec'' H0.
-      eapply lift2_invert_exec in H6; cleanup.
+      eapply lift2_invert_exec in H7; cleanup.
       edestruct H; eauto; cleanup.
       
       do 2 eexists; split.
@@ -224,64 +224,64 @@ Local Lemma lift2_invert_exec_crashed :
 
   Local Ltac invert_exec' :=
     match goal with
-    |[H : recovery_exec _ _ _ _ _ _ _ |- _ ] =>
+    |[H : recovery_exec _ _ _ _ _ _ _ _ |- _ ] =>
      invert_exec'' H
-    | [ H: exec _ _ _ ?p _ |- _ ] =>
+    | [ H: exec _ _ _ _ ?p _ |- _ ] =>
       match p with
       | Bind _ _ => fail
       | Op _ _ => invert_exec'' H
       | Ret _ => invert_exec'' H
       end
-    | [ H: exec' _ _ ?p _ |- _ ] =>
+    | [ H: exec' _ _ _ ?p _ |- _ ] =>
       match p with
       | Bind _ _ => fail
       | Op _ _ => invert_exec'' H
       | Ret _ => invert_exec'' H
       end
-    | [ H: exec _ _ _ (lift_L1 _ _) (Finished _ _) |- _ ] =>
+    | [ H: exec _ _ _ _ (lift_L1 _ _) (Finished _ _) |- _ ] =>
       eapply lift1_invert_exec in H; logic_clean
-    | [ H: exec _ _ _ (lift_L2 _ _) (Finished _ _) |- _ ] =>
+    | [ H: exec _ _ _ _ (lift_L2 _ _) (Finished _ _) |- _ ] =>
       eapply lift2_invert_exec in H; logic_clean
-    | [ H: exec _ _ _ (lift_L1 _ _) (Crashed _) |- _ ] =>
+    | [ H: exec _ _ _ _ (lift_L1 _ _) (Crashed _) |- _ ] =>
       eapply lift1_invert_exec_crashed in H; logic_clean
-    | [ H: exec _ _ _ (lift_L2 _ _) (Crashed _) |- _ ] =>
+    | [ H: exec _ _ _ _ (lift_L2 _ _) (Crashed _) |- _ ] =>
       eapply lift2_invert_exec_crashed in H; logic_clean
-    | [ H: HorizontalComposition.exec' _ _ _ _ |- _ ] =>
+    | [ H: HorizontalComposition.exec' _ _ _ _ _ |- _ ] =>
       invert_exec'' H
-    | [ H: Core.exec _ _ _ _ _ |- _ ] =>
+    | [ H: Core.exec _ _ _ _ _ _ |- _ ] =>
       invert_exec'' H
     end.
 
   Ltac invert_exec :=
   invert_exec' +
   match goal with
-  |[H : exec _ _ _ (Bind _ _) _ |- _ ] =>
+  |[H : exec _ _ _ _ (Bind _ _) _ |- _ ] =>
    apply bind_sep in H; repeat cleanup
-  |[H : exec' _ _ (Bind _ _) _ |- _ ] =>
+  |[H : exec' _ _ _ (Bind _ _) _ |- _ ] =>
    apply bind_sep in H; repeat cleanup
   end.
 
   Ltac invert_exec_no_match :=
   invert_exec' +
   match goal with
-  |[H : exec _ _ _ (Bind _ _) _ |- _ ] =>
+  |[H : exec _ _ _ _ (Bind _ _) _ |- _ ] =>
    apply bind_sep in H; repeat cleanup_no_match
-  |[H : exec' _ _ (Bind _ _) _ |- _ ] =>
+  |[H : exec' _ _ _ (Bind _ _) _ |- _ ] =>
    apply bind_sep in H; repeat cleanup_no_match
   end.
 
   Ltac unify_execs :=
     match goal with
-    |[H : recovery_exec ?x ?y ?z ?a ?b ?c _,
-      H0 : recovery_exec ?x ?y ?z ?a ?b ?c _ |- _ ] =>
+    |[H : recovery_exec ?u ?x ?y ?z ?a ?b ?c _,
+      H0 : recovery_exec ?u ?x ?y ?z ?a ?b ?c _ |- _ ] =>
      eapply recovery_exec_deterministic_wrt_reboot_state in H; [| apply H0]
-    | [ H: exec ?x ?y ?z ?a _,
-        H0: exec ?x ?y ?z ?a _ |- _ ] =>
+    | [ H: exec ?u ?x ?y ?z ?a _,
+        H0: exec ?u ?x ?y ?z ?a _ |- _ ] =>
       eapply exec_deterministic_wrt_oracle in H; [| apply H0]
-    | [ H: exec' ?x ?y ?z _,
-        H0: exec' ?x ?y ?z _ |- _ ] =>
+    | [ H: exec' ?u ?x ?y ?z _,
+        H0: exec' ?u ?x ?y ?z _ |- _ ] =>
       eapply exec_deterministic_wrt_oracle in H; [| apply H0]
-    | [ H: exec _ ?x ?y ?z _,
-        H0: Language.exec' ?x ?y ?z _ |- _ ] =>
+    | [ H: exec _ ?u ?x ?y ?z _,
+        H0: Language.exec' ?u ?x ?y ?z _ |- _ ] =>
       eapply exec_deterministic_wrt_oracle in H; [| apply H0]
     end.
